induction over recursive functions is working, now just needs some pushing

SHA256/MessageSchedule.v
@@ -22,20 +22,34 @@ Require Import Cryptol.Eager.
 
 Require Import Cryptol.Prims.
 Require Import SHA256.SHA256.
-Require Import SHA256.Helpers.
+Require Import SHA256.SS0.
+Require Import SHA256.SS1.
 
 Import HaskellListNotations.
-Definition W_expr : Expr := (EApp
-             (EApp
-              (ETApp
-               (ETApp
+
+Definition W_expr : Expr :=             (EAbs (357,"n")
+             (EIf (EApp
+                   (EApp
+                    (ETApp
+                     (EVar (13,"<"))
+                     (ETyp (TCon (TC TCSeq) [TCon (TC (TCNum 8)) [],TCon (TC TCBit) []])))
+                    (EVar (357,"n")))
+                   (ETApp
+                    (ETApp
+                     (EVar (0,"demote"))
+                     (ETyp (TCon (TC (TCNum 16)) [])))
+                    (ETyp (TCon (TC (TCNum 8)) []))))
+              (EApp
+               (EApp
                 (ETApp
-                 (EVar (34,"#"))
-                 (ETyp (TCon (TC (TCNum 16)) [])))
-                (ETyp (TCon (TC (TCNum 48)) [])))
-               (ETyp (TCon (TC TCSeq) [TCon (TC (TCNum 32)) [],TCon (TC TCBit) []])))
-              (EVar (272,"M")))
-             (EComp
+                 (ETApp
+                  (ETApp
+                   (EVar (40,"@"))
+                   (ETyp (TCon (TC (TCNum 16)) [])))
+                  (ETyp (TCon (TC TCSeq) [TCon (TC (TCNum 32)) [],TCon (TC TCBit) []])))
+                 (ETyp (TCon (TC (TCNum 8)) [])))
+                (EVar (354,"M")))
+               (EVar (357,"n")))
               (EApp
                (EApp
                 (ETApp
@@ -54,42 +68,26 @@ Definition W_expr : Expr := (EApp
                     (EApp
                      (EVar (247,"s1"))
                      (EApp
-                      (EApp
-                       (ETApp
-                        (ETApp
-                         (ETApp
-                          (EVar (40,"@"))
-                          (ETyp (TCon (TC (TCNum 64)) [])))
-                         (ETyp (TCon (TC TCSeq) [TCon (TC (TCNum 32)) [],TCon (TC TCBit) []])))
-                        (ETyp (TCon (TC (TCNum 8)) [])))
-                       (EVar (273,"W")))
+                      (EVar (355,"W"))
                       (EApp
                        (EApp
                         (ETApp
                          (EVar (2,"-"))
                          (ETyp (TCon (TC TCSeq) [TCon (TC (TCNum 8)) [],TCon (TC TCBit) []])))
-                        (EVar (274,"j")))
+                        (EVar (357,"n")))
                        (ETApp
                         (ETApp
                          (EVar (0,"demote"))
                          (ETyp (TCon (TC (TCNum 2)) [])))
                         (ETyp (TCon (TC (TCNum 8)) [])))))))
                    (EApp
-                    (EApp
-                     (ETApp
-                      (ETApp
-                       (ETApp
-                        (EVar (40,"@"))
-                        (ETyp (TCon (TC (TCNum 64)) [])))
-                       (ETyp (TCon (TC TCSeq) [TCon (TC (TCNum 32)) [],TCon (TC TCBit) []])))
-                      (ETyp (TCon (TC (TCNum 8)) [])))
-                     (EVar (273,"W")))
+                    (EVar (355,"W"))
                     (EApp
                      (EApp
                       (ETApp
                        (EVar (2,"-"))
                        (ETyp (TCon (TC TCSeq) [TCon (TC (TCNum 8)) [],TCon (TC TCBit) []])))
-                      (EVar (274,"j")))
+                      (EVar (357,"n")))
                      (ETApp
                       (ETApp
                        (EVar (0,"demote"))
@@ -98,54 +96,32 @@ Definition W_expr : Expr := (EApp
                  (EApp
                   (EVar (246,"s0"))
                   (EApp
-                   (EApp
-                    (ETApp
-                     (ETApp
-                      (ETApp
-                       (EVar (40,"@"))
-                       (ETyp (TCon (TC (TCNum 64)) [])))
-                      (ETyp (TCon (TC TCSeq) [TCon (TC (TCNum 32)) [],TCon (TC TCBit) []])))
-                     (ETyp (TCon (TC (TCNum 8)) [])))
-                    (EVar (273,"W")))
+                   (EVar (355,"W"))
                    (EApp
                     (EApp
                      (ETApp
                       (EVar (2,"-"))
                       (ETyp (TCon (TC TCSeq) [TCon (TC (TCNum 8)) [],TCon (TC TCBit) []])))
-                     (EVar (274,"j")))
+                     (EVar (357,"n")))
                     (ETApp
                      (ETApp
                       (EVar (0,"demote"))
                       (ETyp (TCon (TC (TCNum 15)) [])))
                      (ETyp (TCon (TC (TCNum 8)) []))))))))
                (EApp
-                (EApp
-                 (ETApp
-                  (ETApp
-                   (ETApp
-                    (EVar (40,"@"))
-                    (ETyp (TCon (TC (TCNum 64)) [])))
-                   (ETyp (TCon (TC TCSeq) [TCon (TC (TCNum 32)) [],TCon (TC TCBit) []])))
-                  (ETyp (TCon (TC (TCNum 8)) [])))
-                 (EVar (273,"W")))
+                (EVar (355,"W"))
                 (EApp
                  (EApp
                   (ETApp
                    (EVar (2,"-"))
                    (ETyp (TCon (TC TCSeq) [TCon (TC (TCNum 8)) [],TCon (TC TCBit) []])))
-                  (EVar (274,"j")))
+                  (EVar (357,"n")))
                  (ETApp
                   (ETApp
                    (EVar (0,"demote"))
                    (ETyp (TCon (TC (TCNum 16)) [])))
-                  (ETyp (TCon (TC (TCNum 8)) []))))))
-              [[(From (274,"j") (ETApp
-                                 (ETApp
-                                  (ETApp
-                                   (EVar (49,"fromTo"))
-                                   (ETyp (TCon (TC (TCNum 16)) [])))
-                                  (ETyp (TCon (TC (TCNum 63)) [])))
-                                 (ETyp (TCon (TC (TCNum 8)) []))))]])).
+                  (ETyp (TCon (TC (TCNum 8)) [])))))))).
+
 
 Definition base_case (M : ext_val) (idx : nat) : ext_val :=
   match M with
@@ -157,7 +133,8 @@ Definition base_case (M : ext_val) (idx : nat) : ext_val :=
   | _ => eseq nil
   end.
 
-Fixpoint W_ev (fuel : nat) (M : ext_val) {struct fuel} : ext_val :=
+(* calculate a single element of W, given an M *)
+Fixpoint W_elt_ev (fuel : nat) (M : ext_val) {struct fuel} : ext_val :=
   match fuel with
   (* if idx >= 16 *) 
   | S (S fuel2) =>
@@ -168,10 +145,10 @@ Fixpoint W_ev (fuel : nat) (M : ext_val) {struct fuel} : ext_val :=
         match fuel15 with
         | S fuel16 =>
           (* then (s1 (W@(idx-2)) (W@(idx-7))) + (s0 (W@(j-15)) (W@(j-16))) *)
-          let W2 := W_ev fuel2 M in
-          let W7 := W_ev fuel7 M in
-          let W15 := W_ev fuel15 M in
-          let W16 := W_ev fuel16 M in
+          let W2 := W_elt_ev fuel2 M in
+          let W7 := W_elt_ev fuel7 M in
+          let W15 := W_elt_ev fuel15 M in
+          let W16 := W_elt_ev fuel16 M in
           plus_ev (s1_spec (plus_ev W2 W7)) (s0_spec (plus_ev W15 W16))
         | _ => base_case M fuel
         end
@@ -182,73 +159,118 @@ Fixpoint W_ev (fuel : nat) (M : ext_val) {struct fuel} : ext_val :=
     | _ => base_case M fuel
   end.
 
-Fixpoint ext_to_nat (l : list ext_val) : nat :=
-  match ExtToBitvector.to_bitv l with
-  | Some bv => Z.to_nat (@unsigned (Datatypes.length l) bv)
-  | _ => O
+(* calculate all of W, given a max element *)
+Fixpoint W_ev (fuel : nat) (M : ext_val) : ext_val :=
+  match fuel with
+  | O => eseq nil
+  | S n =>
+    match W_ev n M with
+    | eseq l =>
+      eseq (l ++ [(W_elt_ev n M)])
+    | _ => eseq nil
+    end
   end.
 
+Definition ext_to_nat (l : list ext_val) : option nat :=
+  match ExtToBitvector.to_bitv l with
+  | Some bv => Some (Z.to_nat (@unsigned (Datatypes.length l) bv))
+  | _ => None
+  end.
+
+Definition extnum (val width : Z) : list ext_val :=
+  ExtToBitvector.from_bitv (@repr (Z.to_nat width) val).
+
 (* we can evaluate W @ n to an answer modeled by W_ev *)
-Lemma W_eval :
-  forall n wid GE TE SE,
+Lemma W_eval_inductive :
+  forall GE TE SE,
     wf_env ge GE TE SE ->
-    GE (wid,"W") = Some W_expr ->
-    SE (wid,"W") = None ->
-    forall M idx l,
+    GE (355,"W") = Some (W_expr) ->
+    SE (355,"W") = None ->
+    forall k n M idx l,
+      (n < k)%nat ->
+      SE (354,"M") = Some (to_sval M) ->
+      SE (357,"n") = Some (to_sval (eseq l)) ->
       has_type M (tseq 16 (tseq 32 tbit)) ->
+      has_type (eseq l) (tseq (length l) tbit) ->
       eager_eval_expr GE TE SE idx (to_sval (eseq l)) ->
-      n = ext_to_nat l ->
-      (n <= 64)%nat ->
-      forall ta1 ta2 ta3 tv1 tv2 tv3,
-        eager_eval_type GE TE ta1 tv1 ->
-        eager_eval_type GE TE ta2 tv2 ->
-        eager_eval_type GE TE ta3 tv3 ->
-        forall res,
-        res = to_sval (W_ev n M) ->
-        eager_eval_expr GE TE SE (EApp (EApp (ETApp (ETApp (ETApp (EVar (40,"@")) (ETyp ta1)) (ETyp ta2)) (ETyp ta3)) (EVar (wid,"W"))) idx) res.
+      ext_to_nat l = Some n ->
+      forall res,
+        res = to_sval (W_elt_ev n M) ->
+        eager_eval_expr GE TE SE (EApp (EVar (355,"W")) idx) res.
 Proof.
-Admitted.
-
-
-
-Definition schedule_ev (fuel : nat) (e : ext_val) : ext_val := eseq nil.
-      
-(* This one is fun, since it has a recursive list comprehension in it *)
-Lemma SHA256MessageSchedule_eval :
-  forall n GE TE SE,
-    wf_env ge GE TE SE ->
-    forall a v res,
-      eager_eval_expr GE TE SE a (to_sval v) ->
-      has_type v (tseq 16 (tseq 32 tbit)) ->
-      res = to_sval (schedule_ev n v) ->
-      eager_eval_expr GE TE SE (EApp (EVar SHA256MessageSchedule) a) res.
-Proof.
-  induction n; intros.
-  gen_global SHA256MessageSchedule.
+  intros GE TE SE Hwf HgeW HseW.
+  gen_global (13,"<").
   gen_global (0,"demote").
   gen_global (1,"+").
   gen_global (2,"-").
-  gen_global (34,"#").
-  gen_global (40,"@").
-  gen_global (49,"fromTo").
-(*  inversion H1. subst v t.
-  remember (zrange 16 64) as rng.
-  remember rng as rng2. rewrite Heqrng2 in Heqrng.
-  rewrite Heqrng in Heqrng2.
-  assert (rng = rng2) by congruence.
-  repeat (rewrite zrange_eq in Heqrng;
-          match goal with
-          | [ H : context[Z_lt_dec ?X ?Y] |- _ ] => destruct (Z_lt_dec X Y) eqn:?; try omega; [idtac]
-          end).
-  clear -GE TE SE H a res l rng Heqrng H0 H1 H2 H3 H4 H5 H6 H7 H8 H9 H12 H10 H11 Heqrng2.
-  simpl in Heqrng.
-  e. ag.
-  all: clear H3.
-  e. e. g.*)
-
-
-
+  (* strong induction *)
+  induction k; intros n M idx l Hbound Hm Hn HtypeM HtypeN HevalN Hext_to_nat res Hres; try omega.
   
-  
+  assert (Hcases : (n < 16 \/ n >= 16)%nat) by omega.
+  destruct Hcases.
+
+  * (* base case *)
+    clear IHk.
+    unfold ext_to_nat in *.
+    destruct (ExtToBitvector.to_bitv l) eqn:?; try congruence.
+    inversion Hext_to_nat.
+    e. ag. e. e.
+    use lt_eval.
+    lv.
+    use demote_eval.
+    instantiate (1 := extnum 16 8).
+    reflexivity.
+    assumption.
+    unfold extnum. simpl.
+    repeat (econstructor; eauto).
+    unfold lt_ev. rewrite Heqo. simpl.
+    instantiate (1 := true).
+    destruct (zlt (unsigned b) 16); auto.
+    assert (Z.to_nat 16 <= Z.to_nat (unsigned b))%nat.
+    eapply Z2Nat.inj_le; try omega.
+    rewrite H5 in H4. simpl in H4. unfold Pos.to_nat in *.
+    simpl in *. omega.
+    simpl.
+    subst res.
+    (* TODO: at_eval *)
+    admit.
+    
+  * (* inductive case *)
+    e. ag. e.
+
+    e. instantiate (1 := false).
+    use lt_eval. lv.
+    use demote_eval.
+    instantiate (1 := extnum 16 8).
+    reflexivity.
+    assumption.
+    unfold extnum. simpl.
+    repeat (econstructor; eauto).
+    unfold lt_ev.
+    admit. (* works out *)
+
+    simpl.
+
+    eapply plus_eval.
+    intuition; eassumption.
+    intuition; eassumption.
+    et.
+
+    eapply plus_eval.
+    intuition; eassumption.
+    intuition; eassumption.
+    et.
+
+    eapply plus_eval.
+    intuition; eassumption.
+    intuition; eassumption.
+    et.
+
+    
+    
+    
+    idtac.
 Admitted.
+
+
 
