SHA256/Maj.v
@@ -1,0 +1,69 @@
+Require Import List.
+Import ListNotations.
+
+(* Borrow from CompCert *)
+Require Import Cryptol.Coqlib.
+Require Import Cryptol.Bitvectors.
+
+Require Import Cryptol.AST.
+Require Import Cryptol.Semantics.
+Require Import Cryptol.Utils.
+Require Import Cryptol.Builtins.
+Require Import Cryptol.BuiltinSem.
+Require Import Cryptol.BuiltinSyntax.
+Require Import Cryptol.Values.        
+Require Import Cryptol.Bitstream.
+Require Import Cryptol.Lib.
+Require Import Cryptol.GlobalExtends.
+Require Import Cryptol.GetEachN.
+
+Require Import Cryptol.EvalTac.
+Require Import Cryptol.Eager.
+
+Require Import Cryptol.Prims.
+Require Import SHA256.SHA256.
+
+Definition w32 := tseq 32 tbit.
+
+Definition Maj_spec (x y z : ext_val) : ext_val :=
+  match x,y,z with
+  | eseq x, eseq y, eseq z =>
+    eseq (xor_ev (xor_ev (and_ev x y) (and_ev x z)) (and_ev y z))
+  | _,_,_ => eseq nil
+  end.
+
+Lemma Maj_eval :
+  forall x y z,
+    has_type x w32 ->
+    has_type y w32 ->
+    has_type z w32 ->
+    forall GE TE SE,
+      wf_env ge GE TE SE ->
+      forall ex ey ez res,
+        eager_eval_expr GE TE SE ex (to_sval x) ->
+        eager_eval_expr GE TE SE ey (to_sval y) ->
+        eager_eval_expr GE TE SE ez (to_sval z) ->
+        res = (to_sval (Maj_spec x y z)) ->
+        eager_eval_expr GE TE SE (EApp (EApp (EApp (EVar Maj) ex) ey) ez) res.
+Proof.
+  intros. subst res.
+  gen_global Maj.
+  gen_global (28,"^").
+  gen_global (26,"&&").
+  e. e. e. ag.
+  e. e. e.
+  unfold w32 in *.
+  inversion H. inversion H0. inversion H1. subst.
+  use xor_eval. use xor_eval.
+  use and_eval; try lv; try reflexivity; try eassumption.
+  use and_eval; try lv; try reflexivity; try eassumption.
+  reflexivity. eapply has_type_and; eauto.
+  eapply has_type_and; eauto.
+  use and_eval; try lv; try reflexivity; try eassumption.
+  simpl. reflexivity.
+  eapply has_type_xor.
+  eapply has_type_and. eassumption.
+  eassumption.
+  eapply has_type_and; eassumption.
+  eapply has_type_and; eassumption.
+Qed.
